Complete evaluate logic/concept

RelationalAlgebra/FOL/Evaluate.lean
@@ -7,15 +7,22 @@ open FOL FirstOrder Language RM Term
 
 namespace FOL
 
-def Query.evaluateT [folStruc] {q : FOL.Query} (dbi : DatabaseInstance) : Set Tuple :=
-  {t | q.RealizeDom dbi t}
+def Query.evaluateT [folStruc] (q : FOL.Query) (dbi : DatabaseInstance) : Set Tuple :=
+  {t | ∃ov : Tuple, ∃(h' : ↑q.schema ⊆ ov.Dom), q.RealizeDom dbi (ov.restrict h') ∧ t = (ov.restrict h')}
 
 @[simp]
-theorem realize_query_dom {t : Attribute →. Value} [folStruc] {q : Query} (dbi : DatabaseInstance) (h_wt : q.isWellTyped) (h_realize : q.RealizeDom dbi t) :
+theorem realize_query_dom {t : Attribute →. Value} [folStruc] {q : Query} (dbi : DatabaseInstance) (h_wt : q.isWellTyped) (h_realize : t ∈ q.evaluateT dbi) :
   t.Dom = q.schema := by
     ext a
-    simp only [PFun.Dom, Query.RealizeDom.isWellTyped_def q h_wt (by simp_all; exact h_realize.1),
-      Finset.setOf_mem, Finset.mem_coe, BoundedQuery.isWellTyped.schema_eq_attributesInQuery h_wt]
+    simp_all [PFun.mem_dom, BoundedQuery.isWellTyped.schema_eq_attributesInQuery, Finset.mem_coe, Query.evaluateT]
+    obtain ⟨w, h⟩ := h_realize
+    obtain ⟨w_1, h⟩ := h
+    obtain ⟨left, right⟩ := h
+    subst right
+    simp_all only [PFun.mem_restrict, BoundedQuery.isWellTyped.schema_eq_attributesInQuery, Finset.mem_coe,
+      exists_and_left, and_iff_left_iff_imp]
+    intro a_1
+    exact Part.dom_iff_mem.mp (w_1 a_1)
 
 def Query.evaluate [folStruc] {q : Query} (h : q.isWellTyped) (dbi : DatabaseInstance)
   : RelationInstance := ⟨q.schema, q.evaluateT dbi, λ _ ht ↦ realize_query_dom dbi h ht⟩
