RelationalAlgebra/FOL/Realize.lean
@@ -7,6 +7,43 @@ open FOL FirstOrder Language RM Term
 
 namespace FOL
 
+def Term.realizeSome [folStruc] {n : ℕ} (t : fol.Term (Attribute ⊕ (Fin n))) (ov : Attribute →. Value) (iv : Fin n →. Value) : Prop
+  := (t.realize (Sum.elim ov iv)).Dom
+
+@[simp]
+theorem Term.realizeSome.def [folStruc] (t : fol.Term (Attribute ⊕ (Fin n))) (ov : Attribute →. Value) (iv : Fin n →. Value) :
+  Term.realizeSome t ov iv ↔ (t.realize (Sum.elim ov iv)).Dom := by rfl
+
+-- Formal realization definition, requires all terms to be 'some'
+def BoundedQuery.RealizeTerms {n : ℕ} [folStruc] : BoundedQuery n → (Attribute →. Value) → (Fin n →. Value) → Prop
+  | R dbs rn t, ov, iv => (∀i, Term.realizeSome (t i) ov iv) ∧ (R dbs rn t).toFormula.Realize ov iv
+  | tEq q t₁ t₂, ov, iv => q.RealizeTerms ov iv ∧ Term.realizeSome t₁ ov iv ∧ Term.realizeSome t₂ ov iv ∧ (BoundedFormula.equal t₁ t₂).Realize ov iv
+  | and q₁ q₂, ov, iv => q₁.RealizeTerms ov iv ∧ q₂.RealizeTerms ov iv
+  | ex q, ov, iv => ∃a, q.RealizeTerms ov (Fin.snoc iv a)
+
+@[simp]
+theorem BoundedQuery.RealizeTerms.R_def [folStruc] {n : ℕ} (t) {ov : Attribute →. Value} {iv : Fin n →. Value}
+  : (R dbs rn t).RealizeTerms ov iv ↔ (∀i, Term.realizeSome (t i) ov iv) ∧ (R dbs rn t).toFormula.Realize ov iv := by
+    rfl
+
+@[simp]
+theorem BoundedQuery.RealizeTerms.tEq_def [folStruc] {n : ℕ} (q : BoundedQuery n) (t₁ t₂ : fol.Term (Attribute ⊕ Fin n)) {ov : Attribute →. Value} {iv : Fin n →. Value}
+  : (tEq q t₁ t₂).RealizeTerms ov iv ↔ (q.RealizeTerms ov iv ∧ Term.realizeSome t₁ ov iv ∧ Term.realizeSome t₂ ov iv ∧ (BoundedFormula.equal t₁ t₂).Realize ov iv) := by
+    rfl
+
+@[simp]
+theorem BoundedQuery.RealizeTerms.and_def [folStruc] {n : ℕ} (q₁ q₂ : BoundedQuery n) {ov : Attribute →. Value} {iv : Fin n →. Value}
+  : (and q₁ q₂).RealizeTerms ov iv ↔ q₁.RealizeTerms ov iv ∧ q₂.RealizeTerms ov iv := by
+    rfl
+
+@[simp]
+theorem BoundedQuery.RealizeTerms.ex_def [folStruc] {n : ℕ} (q : BoundedQuery (n + 1)) {ov : Attribute →. Value} {iv : Fin n →. Value}
+  : (ex q).RealizeTerms ov iv ↔ ∃a, q.RealizeTerms ov (Fin.snoc iv a) := by
+    rfl
+
+theorem Term.cases [folStruc] (t : fol.Term (Attribute ⊕ (Fin n))) : ∃k, t = var k := by
+  cases t with | var k => use k | func _f _ => exact False.elim (folStruc_empty_fun _f)
+
 def BoundedQuery.RealizeValidDom (q : BoundedQuery n) (dbi : DatabaseInstance) (ov : Tuple) (iv : Fin n →. Value) : Prop :=
   (∀a ∈ q.attributesInQuery, (ov a).Dom) ∧ (ov.ran ⊆ dbi.domain) ∧ (∀i : Fin n, (iv i).Dom) ∧ (iv.ran ⊆ dbi.domain)
 
@@ -29,75 +66,57 @@ theorem BoundedQuery.Realize.def [folStruc] {n : ℕ} (q : BoundedQuery n) {ov :
 
 -- Realize a bounded query considering the database domain, using Attribute and Fin n maps
 def BoundedQuery.RealizeDom {n : ℕ} (dbi : DatabaseInstance) [folStruc] : BoundedQuery n → (Attribute →. Value) → (Fin n →. Value) → Prop
-  -- | ex q, ov, iv  => (∃a iv', iv' = (Fin.snoc iv a) ∧ q.Realize ov iv' ∧ ov.ran ⊆ dbi.domain ∧ (PFun.ran iv') ⊆ dbi.domain)
-  | q, ov, iv     => q.Realize ov iv ∧ q.RealizeValidDom dbi ov iv
+  | q, ov, iv     => q.RealizeTerms ov iv ∧ q.RealizeValidDom dbi ov iv
 
 @[simp]
 theorem BoundedQuery.RealizeDom.def [folStruc] {q : BoundedQuery n} :
-  q.RealizeDom dbi ov iv ↔ q.Realize ov iv ∧ q.RealizeValidDom dbi ov iv := by rfl
+  q.RealizeDom dbi ov iv ↔ q.RealizeTerms ov iv ∧ q.RealizeValidDom dbi ov iv := by rfl
 
 -- Realize a query considering the database domain, using just an Attribute
-nonrec def Query.RealizeDom (φ : Query) (dbi : DatabaseInstance) [folStruc] (v : Attribute → Part Value) : Prop :=
-  φ.RealizeDom dbi v (λ _ => .none)
+nonrec def Query.RealizeDom (φ : Query) (dbi : DatabaseInstance) [folStruc] (v : Attribute →. Value) : Prop :=
+  φ.RealizeDom dbi v default ∧ v.Dom = φ.attributesInQuery
 
 @[simp]
 theorem Query.RealizeDom.def [folStruc] (φ : Query)
-  : φ.RealizeDom dbi ov = BoundedQuery.RealizeDom dbi φ ov (λ _ => .none) := rfl
+  : φ.RealizeDom dbi ov ↔ BoundedQuery.RealizeDom dbi φ ov default ∧ ov.Dom = φ.attributesInQuery := by rfl
 
 @[simp]
-theorem Query.RealizeDom.isWellTyped_def {iv : Fin n →. Value} [folStruc] (φ : BoundedQuery n) (h : φ.isWellTyped) (h' : φ.Realize t iv) :
- (t a).Dom ↔ a ∈ BoundedQuery.attributesInQuery φ := by
-    simp_all
+theorem Query.RealizeDom.isWellTyped_def {iv : Fin n →. Value} [folStruc] (φ : BoundedQuery n) (h : φ.isWellTyped) (h' : φ.RealizeTerms t iv) :
+ a ∈ BoundedQuery.attributesInQuery φ → (t a).Dom := by
     induction φ with
     | R =>
       aesop
-      . --have ⟨dbi, h_dbi, ht⟩ := folStruc_apply_RelMap h'
-        -- have z' := (dbi.relations rn).validSchema_def ht
-        -- simp_all [dbi.validSchema]
-        -- subst h_dbi
-        -- have z'' : a ∈ (dbi.schema rn) ↔ a ∈ PFun.Dom (ArityToTuple fun i ↦ realize (Sum.elim t iv) (a_1 i)) := by simp_all
-        -- have z''' : a ∈ PFun.Dom (ArityToTuple fun i ↦ realize (Sum.elim t iv) (a_1 i)) := by
-        --   simp [Part.dom_iff_mem, ← Part.eq_some_iff]
-        --   use (t a).get a_2
-        --   simp_all
-        --   unfold ArityToTuple at *
-        --   by_cases hc : a ∈ dbs rn
-        --   . have z := RelationSchema.index?_isSome.mpr hc
-        --     simp [Option.isSome_iff_exists] at z
-        --     obtain ⟨w, h_2⟩ := z
-        --     simp_all only [Option.map_some', Option.getD_some]
-        --     have z' := h w
-
-        --   . have z := RelationSchema.index?_none.mpr hc
-        --     rw [z]
-        --     aesop
-        -- simp_all
-        sorry
-      . sorry --@TODO: Achieve this, possibly by changing the folStruc/isWellTyped concept
+      have z := Term.cases (a_1 w)
+      aesop
+      have z' := left w
+      aesop
     | tEq sq t₁ t₂ sq_ih =>
       simp_all
-      simp_all [sq_ih h'.1]
       intro a_1
       obtain ⟨left, right⟩ := h
       obtain ⟨left_1, right_1⟩ := h'
       simp_all only [BoundedQuery.isWellTyped.schema_eq_attributesInQuery]
-      cases a_1 with
-      | inl h =>
-        apply right
-        simp_all only [Finset.mem_union, true_or]
-      | inr h_1 =>
-        apply right
-        simp_all only [Finset.mem_union, or_true]
-    | _ => aesop
+      aesop
+    | and => aesop
+    | ex q q_ih => aesop
 
 @[simp]
-theorem Query.RealizeDom.isWellTyped_eq_Realize [folStruc] (φ : Query) (h : t ∈ (dbi.relations rn).tuples) (h' : φ.isWellTyped) :
- φ.RealizeDom dbi t = φ.Realize t (λ _ => .none) := by
-    simp_all
-    intros h''
-    apply And.intro
-    . intros a h
-      exact (isWellTyped_def φ h' h'').mpr h
-    . apply And.intro
-      . exact DatabaseInstance.t_ran_sub_domain h
-      . simp_all [PFun.ran]
+theorem Query.RealizeDom.isWellTyped_eq_Realize [folStruc] (φ : Query) (h : t ∈ (dbi.relations rn).tuples) (h' : φ.isWellTyped) (h'' : t.Dom = ↑φ.schema) :
+ φ.RealizeDom dbi t = φ.RealizeTerms t default := by
+    simp_all only [«def», BoundedQuery.RealizeDom.def, BoundedQuery.RealizeTerms,
+      BoundedQuery.RealizeValidDom.def, zero_le, Part.not_none_dom, IsEmpty.forall_iff, true_and,
+      eq_iff_iff, and_iff_left_iff_imp, and_imp]
+    apply Iff.intro
+    · intro a
+      simp_all only
+    · intro h''
+      simp_all only [true_and]
+      apply And.intro
+      · apply And.intro
+        · intro a h
+          exact isWellTyped_def φ h' h'' h
+        · apply And.intro
+          · exact DatabaseInstance.t_ran_sub_domain h
+          · simp_all [PFun.ran]
+      · simp_all only [(dbi.relations rn).validSchema, DatabaseInstance.validSchema_def,
+        BoundedQuery.isWellTyped.schema_eq_attributesInQuery, Finset.coe_inj]
